Update Hacl.Hash.Core.Blake2 to make the definitions generic in the algorithm

code/hash/Hacl.Hash.Core.Blake2.fst
@@ -3,6 +3,7 @@ module Hacl.Hash.Core.Blake2
 open Lib.IntTypes
 
 module B = LowStar.Buffer
+module HS = FStar.HyperStack
 module ST = FStar.HyperStack.ST
 module M = LowStar.Modifies
 
@@ -14,56 +15,49 @@ friend Spec.Agile.Hash
 
 #push-options "--ifuel 0 --fuel 0"
 
-let alloca_blake2s () =
+noextract inline_for_extraction
+val mk_init (a:hash_alg{is_blake a}) : init_st a
+
+let mk_init a s =
+  Impl.blake2_init_hash #(to_blake_alg a) #Core.M32 s (size 0)
+                        (size (Spec.max_output (to_blake_alg a)));
+  nat_to_extra_state a 0
+
+noextract inline_for_extraction
+val mk_alloca (a:hash_alg{is_blake a}) : init_st a -> alloca_st a
+
+let mk_alloca a init () =
   let h0 = ST.get() in
-  let (s:Core.state_p Spec.Blake2S Core.M32) = Lib.Buffer.create 16ul (u32 0) in
-  Impl.blake2_init_hash #Spec.Blake2S #Core.M32 s (size 0) (size 32);
+  let (s:Core.state_p (to_blake_alg a) Core.M32) =
+    Lib.Buffer.create (4ul *. Core.row_len (to_blake_alg a) Core.M32)
+                      (Core.zero_element (to_blake_alg a) Core.M32) in
+  let es = init s in
   let h2 = ST.get() in
   B.modifies_only_not_unused_in (B.loc_none) h0 h2;
-  s, (u64 0)
+  assert((as_seq h2 s, es) == Spec.Agile.Hash.init a);
+  (s <: state a), es
 
-let init_blake2s s =
-  Impl.blake2_init_hash #Spec.Blake2S #Core.M32 s (size 0) (size 32);
-  (u64 0)
+noextract inline_for_extraction
+val mk_update (a:hash_alg{is_blake a}) : update_st a
 
-let update_blake2s s totlen block =
+let mk_update a s totlen block =
   ST.push_frame();
-  let wv = Lib.Buffer.create 16ul (u32 0) in
-  let totlen = totlen +. u64 64 in
-  Impl.blake2_update_block #Spec.Blake2S #Core.M32 wv s false totlen block;
-  assert (64 == size_block Blake2S);
+  let (wv:Core.state_p (to_blake_alg a) Core.M32) =
+    Lib.Buffer.create (4ul *. Core.row_len (to_blake_alg a) Core.M32)
+                      (Core.zero_element (to_blake_alg a) Core.M32) in
+  let totlen = extra_state_add_size_t totlen (block_len a) in
+  Impl.blake2_update_block #(to_blake_alg a) #Core.M32 wv s false totlen block;
   ST.pop_frame();
   totlen
 
+let init_blake2s = mk_init Blake2S
+let alloca_blake2s = mk_alloca Blake2S (mk_init Blake2S)
+let update_blake2s = mk_update Blake2S
 let pad_blake2s = Hacl.Hash.PadFinish.pad Blake2S
-
 let finish_blake2s = Hacl.Hash.PadFinish.finish Blake2S
 
-let alloca_blake2b () =
-  let h0 = ST.get() in
-  let (s:Core.state_p Spec.Blake2B Core.M32) = Lib.Buffer.create 16ul (u64 0) in
-  Impl.blake2_init_hash #Spec.Blake2B #Core.M32 s (size 0) (size 64);
-  let h2 = ST.get() in
-  B.modifies_only_not_unused_in (B.loc_none) h0 h2;
-  s, (nat_to_extra_state Blake2B 0)
-
-let init_blake2b s =
-  Impl.blake2_init_hash #Spec.Blake2B #Core.M32 s (size 0) (size 64);
-  nat_to_extra_state Blake2B 0
-
-#push-options "--z3rlimit 20"
-
-let update_blake2b s totlen block =
-  ST.push_frame();
-  let wv = Lib.Buffer.create 16ul (u64 0) in
-  let totlen = totlen +. u128 128 in
-  Impl.blake2_update_block #Spec.Blake2B #Core.M32 wv s false (to_u128 totlen) block;
-  assert (128 == size_block Blake2B);
-  ST.pop_frame();
-  totlen
-
-#pop-options
-
+let init_blake2b = mk_init Blake2B
+let alloca_blake2b = mk_alloca Blake2B (mk_init Blake2B)
+let update_blake2b = mk_update Blake2B
 let pad_blake2b = Hacl.Hash.PadFinish.pad Blake2B
-
 let finish_blake2b = Hacl.Hash.PadFinish.finish Blake2B
