code/hash/Hacl.Hash.Core.Blake2.fsti
@@ -4,15 +4,20 @@ open Hacl.Hash.Definitions
 open Spec.Hash.Definitions
 
 noextract inline_for_extraction
-val alloca_blake2s: alloca_st Blake2S
+val mk_init (a:hash_alg{is_blake a}) : init_st a
+val mk_alloca (a:hash_alg{is_blake a}) : init_st a -> alloca_st a
+val mk_update (a:hash_alg{is_blake a}) : update_st a
+
+noextract inline_for_extraction
 val init_blake2s: init_st Blake2S
+val alloca_blake2s: alloca_st Blake2S
 val update_blake2s: update_st Blake2S
 val pad_blake2s: pad_st Blake2S
 val finish_blake2s: finish_st Blake2S
 
 noextract inline_for_extraction
-val alloca_blake2b: alloca_st Blake2B
 val init_blake2b: init_st Blake2B
+val alloca_blake2b: alloca_st Blake2B
 val update_blake2b: update_st Blake2B
 val pad_blake2b: pad_st Blake2B
 val finish_blake2b: finish_st Blake2B
